programs/lean/Project/SwapElementsOpt3/SmallStepEquivalence.lean
@@ -260,7 +260,7 @@ theorem opt3_func0_distinct_store_partiallyMeets
     simpa using UInt32.add_ofNat_toNat_noWrap addressJ 7 (by omega) (by omega)
   apply
     Wasm.SmallStep.wasm_smallStep_heap_globals_runtime_store_partiallyMeets.{0}
-      (α := Unit) (σ := σ) (globalσ := globalσ)
+      (α := Unit) (σ := σ) (globalσ := globalσ) (hhost := trivial)
   · exact hagree
   · exact hinBounds
   · exact hglobals
